cem.v
@@ -1,19 +1,20 @@
-Require Import expr_db_nat.
+Require Import expr_db_nat util.
 Require Import Arith.EqNat.
 Require Import List Unicode.Utf8.
+Require Import CpdtTactics.
 
 Definition append := Datatypes.app.
 
 Inductive closure : Type := 
-  | close : expr -> nat -> closure. 
+  | close : expr → nat → closure. 
 
 Inductive cell : Type :=
-  | cl : closure -> nat -> cell.
+  | cl : closure → nat → cell.
 
 Definition heap := list (nat * cell).
 
 Inductive configuration : Type :=
-  | st : heap -> closure -> configuration.
+  | st : heap → closure → configuration.
 
 Notation " x ↦ M " := (x, M) (at level 40).
 Notation " ⟨ Φ ⟩ m " := (st Φ m) (at level 40).
@@ -22,9 +23,9 @@ Notation " ⟨ Φ , b , Ψ ⟩ N " := (st (append _ Ψ (cons b Φ)) N) (at level
 Notation " { M , e } " := (cl M e).
 Notation " < M , e > " := (close M e).
 
-Inductive cactus_lookup : nat -> nat -> heap -> nat -> Prop :=
+Inductive cactus_lookup : nat → nat → heap → nat → Prop :=
   | zero : forall x Φ M Υ, cactus_lookup 0 x (append _ Φ (cons (x ↦ M) Υ)) x
-  | pred : forall x y z Φ M Υ i, cactus_lookup i x Φ z -> 
+  | pred : forall x y z Φ M Υ i, cactus_lookup i x Φ z → 
             cactus_lookup (S i) y (append _ Φ (cons (y ↦ {M, x}) Υ)) z.
 
 Definition lookup {a} (x:nat) (l:list (nat * a)) : option a := 
@@ -43,14 +44,8 @@ Fixpoint clu (v env:nat) (h:heap) : option nat := match v with
 
 Definition domain (h:heap) : list nat := @map (nat * cell) nat (@fst nat cell) h.
 
-Definition fresh (n : nat) (h : heap) (d : list nat) := 
-  ~ In n d
-  /\ ~ In n (domain h).
-
-Fixpoint forevery {a} (l:list a) (p : a → Prop) : Prop := match l with
-  | cons x xs => p x ∧ forevery xs p
-  | nil => True
-  end.
+Definition fresh (n : nat) (h : heap) := 
+  ~ In n (domain h).
 
 Definition closed_under (c : configuration) : Prop := match c with
   | st h (close t e) => forevery (fvs t) 
@@ -59,31 +54,55 @@ Definition closed_under (c : configuration) : Prop := match c with
 
 Definition closed (t : expr) : Prop := closed_under (st nil (close t 0)).
 
-Fixpoint well_formed_heap (h : heap) : Prop := forevery h 
+Definition well_formed_heap (h : heap) : Prop := forevery h 
   (λ x, match x with | (v,cl c e) => closed_under (st h c) end). 
 
 Definition well_formed (c : configuration) : Prop := match c with 
   | st h t => closed_under c ∧ well_formed_heap h 
   end.
 
-Reserved Notation " c1 '⇓' d '#' c2 " (at level 50).
-Inductive step : configuration -> list nat -> configuration -> Prop :=
-  | Id : ∀ M B x y z Φ Ψ Υ v e d, 
-          cactus_lookup v z (Υ ++ (x ↦ {M,y} :: Φ)) x -> 
-                ⟨Φ⟩M ⇓ cons x (domain Υ ++ d) # ⟨Ψ⟩close (:λB) e ->
-    ⟨Φ, x ↦ {M, y}, Υ⟩close (var v) z ⇓ d # ⟨Ψ, x ↦ {close (:λB) e, y}, Υ⟩close (:λB) e
-  | Abs : ∀ N Φ e d, ⟨Φ⟩close (:λN) e ⇓ d # ⟨Φ⟩close (:λN) e
-  | App : ∀ N M B B' Φ Ψ Υ f e ne ae d, 
-              fresh f Ψ d ->
-          ⟨Φ⟩close M e ⇓ d # ⟨Ψ⟩close (:λB) ne ->
-      ⟨Ψ, f ↦ {close N e, ne}⟩close B f ⇓ d # ⟨Υ⟩close (:λB') ae  -> 
-              ⟨Φ⟩close (M@N) e ⇓ d # ⟨Υ⟩close (:λB') ae
-where " c1 '⇓' d '#' c2 " := (step c1 d c2).
+Reserved Notation " c1 '⇓' c2 " (at level 50).
+Inductive step : configuration → configuration → Prop :=
+  | Id : ∀ M B x y z Φ Ψ Υ v e, 
+                  cactus_lookup v z (Υ ++ (x ↦ {M,y} :: Φ)) x →
+              ⟨Φ, (x ↦ {M,y}), Υ⟩M ⇓ ⟨Ψ, (x ↦ {M,y}), Υ⟩close (:λB) e →
+    ⟨Φ, x ↦ {M, y}, Υ⟩close (var v) z ⇓ ⟨Ψ, x ↦ {close (:λB) e, y}, Υ⟩close (:λB) e
+  | Abs : ∀ N Φ e, ⟨Φ⟩close (:λN) e ⇓ ⟨Φ⟩close (:λN) e
+  | App : ∀ N M B B' Φ Ψ Υ f e ne ae, fresh f Ψ → 
+          ⟨Φ⟩close M e ⇓ ⟨Ψ⟩close (:λB) ne → 
+      ⟨Ψ, f ↦ {close N e, ne}⟩close B f ⇓ ⟨Υ⟩close (:λB') ae   →
+              ⟨Φ⟩close (M@N) e ⇓ ⟨Υ⟩close (:λB') ae
+where " c1 '⇓' c2 " := (step c1 c2).
 
-Lemma values_only : ∀ c e M Ψ d, c ⇓ d # ⟨Ψ⟩close M e -> value M.
+Lemma well_formed_inf : ∀ c x c' n  Φ Υ, well_formed (⟨Φ, x ↦ cl c' n, Υ⟩c) → 
+  well_formed (⟨Φ, x ↦ cl c' n, Υ⟩c').
+  intros. split. inversion H. unfold well_formed_heap in H1. apply forevery_app in H1.
+  destruct H1. simpl in H2. destruct H2. auto. 
+  auto. inversion H. auto. Qed. 
+
+(*
+TODO
+Lemma cactus_lookup_inf : ∀ v x y m n e Φ Υ, cactus_lookup v x (Φ ++ (y ↦ {m, n}) :: Υ) e → ∀ M, cactus_lookup v x (Φ ++ (y ↦ {M, n}) :: Υ) e.
+intros. 
+
+Lemma inf_well_formed : ∀ c x c' n  Φ Υ, well_formed (⟨Φ, x ↦ cl c' n, Υ⟩c) → 
+  well_formed (⟨Φ, x ↦ cl c n, Υ⟩c).
+  intros. inversion H. split. induction Υ. simpl. destruct c. induction (fvs e).
+  simpl. auto. simpl. 
+  destruct (eq_nat_dec x n0). simpl. unfold domain. rewrite
+  map_app. simpl. unfold domain in H0. rewrite map_app in H0. simpl in H0. 
+  kapply forevery_app in H1. destruct H1. simpl in
+  H2. destruct H2. unfold closed_under in H0. clear H1 H2 H3.  (inversion H. apply forevery_app in H1.
+  auto. inversion H. auto. Qed. 
+
+Theorem well_formed_step : ∀ c v, well_formed c → c ⇓ v → well_formed v.
+intros. induction H0. apply well_formed_inf in H. apply IHstep in H.  
+*)
+
+Lemma values_only : ∀ c e M Ψ, c ⇓ ⟨Ψ⟩close M e → value M.
 intros. inversion H; simpl; auto. Qed.
 
-Example simple : (step (⟨nil⟩ close (:λ0 @ :λ0) 0) nil (⟨nil, 0 ↦ {close (:λ0) 0,
+Example simple : (step (⟨nil⟩ close (:λ0 @ :λ0) 0) (⟨nil, 0 ↦ {close (:λ0) 0,
 0}⟩ close (:λ0) 0)).
 apply App with 0 nil 0 0.
 unfold fresh. simpl.  auto. 
@@ -93,4 +112,5 @@ apply Id.
 apply zero.
 apply Abs. 
 Qed.
+
 
