compiler.v
@@ -1,0 +1,28 @@
+Require expr expr_db_nat.
+Require Import db util assembly.
+Require Import Arith.Peano_dec.
+Require Import List Datatypes.
+
+(* Function instead of logical relation, not equivalent! Function takes first
+value in environment, logical relation takes any. Logical relation wrong? *)
+
+Fixpoint db (tm : expr.tm) (env : list (nat * nat)) : option expr_db_nat.expr := match tm with 
+  | expr.var v => match lookup eq_nat_dec v env with
+    | Some v' => Some (expr_db_nat.var v')
+    | None => None
+    end
+  | expr.abs v b => match db b ((v, 0):: map (fmap' S) env) with 
+    | Some b' => Some (expr_db_nat.lam b')
+    | None => None
+    end
+  | expr.app m n => match db m env with
+    | Some m' => match db n env with 
+      | Some n' => Some (expr_db_nat.app m' n')
+      | None => None
+      end
+    | None => None
+    end
+  end.
+
+(* TODO: Assembler from db terms.
+Fixpoint assemble (e : expr_db_nat.expr) : program. *)
